src/MiscFacts.v
@@ -1,0 +1,43 @@
+Require Import Setoid.
+Require Import IndefiniteDescription.
+
+
+Lemma ex_iff_ex:
+  forall T (P Q : T -> Prop),
+    (forall x, P x <-> Q x) ->
+    ex P <-> ex Q.
+Proof.
+  intuition.
+  - destruct H0 as [witness H0].
+    exists witness.
+    apply H.
+    easy.
+  - destruct H0 as [witness H0].
+    exists witness.
+    apply H.
+    easy.
+Qed.
+
+Lemma all_iff_all:
+  forall T (P Q : T -> Prop),
+    (forall x, P x <-> Q x) ->
+    all P <-> all Q.
+Proof.
+  unfold all.
+  intros.
+  setoid_rewrite H.
+  reflexivity.
+Qed.
+
+Lemma forall_exists_to_exists_forall:
+  forall T U (P : T -> U -> Prop),
+    (forall (x:T), exists (y:U), P x y) <->
+    (exists (f : T -> U), forall (x:T), P x (f x)).
+Proof.
+  intuition.
+  - apply functional_choice.
+    easy.
+  - destruct H as [f H].
+    exists (f x).
+    easy.
+Qed.
